theories/CTree/Events/Net.v
@@ -3,94 +3,99 @@ From CTree Require Import
   CTree.Core.
 
 From CTree Require Export
+  CTree.Core
+  Events.Core
   Events.WriterE
   Events.NetE.
 
 From Equations Require Import Equations.
 
+Import CTreeNotations.
+Local Open Scope ctree_scope.
 Local Open Scope fin_vector_scope.
 
 Definition send {n T}: fin' n -> T -> ctree (netE n T) unit :=
   fun i p => Ctree.trigger (Send i p).
 
 Definition recv {n T}: ctree (netE n T) (option T) :=
-  Ctree.trigger Recv.
+  Ctree.trigger (@Recv n T).
 
-Notation retry := (Ret (inl tt)).
-Notation exit := (Ret (inr tt)).
-
-
-(* Round-robbin Scheduler for infinite ctrees, based on message passing.
+Module MessageOrderScheduler.
+  (* Round-robbin Scheduler for infinite ctrees, based on message passing.
    1. Pick non-deterministically an [i: fin n], schedule process [i].
    2. When [i] sends a message to [j], deliver message and schedule [j] next.
    3. Repeat (2).
- *)
+   *)
+  Record Task (n: nat) (T: Type) :=
+    {
+      prog: ctree (netE n T) void;
+      mail: option T
+    }.
+  Arguments prog {n} {T}.
+  Arguments mail {n} {T}.
 
-Record Task (n: nat) (T: Type) :=
-  {
-    prog: ctree (netE n T) void;
-    mail: option T
-  }.
-Arguments prog {n} {T}.
-Arguments mail {n} {T}.
+  Definition task_new {n T}(p: ctree (netE n T) void) :=
+    {| prog := p; mail := None |}.
+  
+  Definition uprog{n T}(p: ctree (netE n T) void)(t: Task n T) :=
+    {| prog := p; mail := t.(mail) |}.
 
-Definition uprog{n T}(p: ctree (netE n T) void)(t: Task n T) :=
-  {| prog := p; mail := t.(mail) |}.
+  Definition umail{n T}(mail: option T) (t: Task n T) :=
+    {| prog := t.(prog); mail := mail |}.
 
-Definition umail{n T}(mail: option T) (t: Task n T) :=
-  {| prog := t.(prog); mail := mail |}.
+  Notation sys n T := (vec' n (Task n T)).
 
-Notation sys n T := (vec' n (Task n T)).
-
-Section ScheduleMsg.
   (* n: Number of processes
-     T: Message payload type
-     W: Observation domain *)
-  Context {n: nat} {T W: Type} (fobs: bool -> fin' n -> option T -> option W).
-  Notation logE := (writerE W).
-  
-  Equations schedule_one' (R: fin' n -> sys n T -> ctree logE void)
-    (r: fin' n) (system: sys n T) : ctree logE void :=
-  
-    schedule_one' R r system with observe (prog (system $ r)) => {
-        (** A non-deterministic choice, traverse it *)
-        schedule_one' _ _ _ (BrF n' k) :=
-          Br n' (fun i => R r (system @ r do uprog (k i)));
+   T: Message payload type
+   W: Observation domain *)
+  Section ScheduleMsg.
+    Context {n: nat} {T W: Type} (fobs: bool -> fin' n -> option T -> option W).
+    Notation logE := (writerE W).
+    
+    Equations schedule_one' (R: fin' n -> sys n T -> ctree logE void)
+      (r: fin' n) (system: sys n T) : ctree logE void :=
+      
+      schedule_one' R r system with observe (prog (system $ r)) => {
+          (** A non-deterministic choice, traverse it *)
+          schedule_one' _ _ _ (BrF n' k) :=
+            Br n' (fun i => R r (system @ r do uprog (k i)));
 
-        (** A guard, traverse it *)
-        schedule_one' _ _ _ (GuardF t') :=
-          Guard (R r (system @ r do uprog t'));
-        
-        (** A network `send` effect, interpet it and context switch *)
-        schedule_one' _ _ _ (VisF (Send to m) k) :=
-          match fobs true to (Some m) with
-          | Some obs =>          
-              Vis (Log obs) (fun _: unit =>
-                               R to (system
-                                       @ r do (uprog (k tt))
-                                                @ to do (umail (Some m))))
-          | None => R to (system @ r do (uprog (k tt)) @ to do (umail (Some m)))
-          end;
-        
-        (** Receive a message *)
-        schedule_one' _ _ _ (VisF Recv k) :=
-          let m := mail (system $ r) in
-          match fobs false r m with
-          | Some obs =>          
-              Vis (Log obs) (fun _: unit => R r (system @ r do (fun t => umail None (uprog (k m) t))))
-          | None => R r (system @ r do (fun t => umail None (uprog (k m) t)))
-          end;
-      }.    
+          (** A guard, traverse it *)
+          schedule_one' _ _ _ (GuardF t') :=
+            Guard (R r (system @ r do uprog t'));
+          
+          (** A network `send` effect, interpet it and context switch *)
+          schedule_one' _ _ _ (VisF (Send to m) k) :=
+            match fobs true to (Some m) with
+            | Some obs =>      
+                Vis (Log obs) (fun _: unit =>
+                                 R to (system
+                                         @ r do (uprog (k tt))
+                                                  @ to do (umail (Some m))))
+            | None => R to (system
+                             @ r do (uprog (k tt))
+                                      @ to do (umail (Some m)))
+            end;
+          
+          (** Receive a message *)
+          schedule_one' _ _ _ (VisF Recv k) :=
+            let m := mail (system $ r) in
+            match fobs false r m with
+            | Some obs =>          
+                Vis (Log obs) (fun _: unit =>
+                                 R r (system @ r do (fun t => umail None (uprog (k m) t))))
+            | None => R r
+                       (system @ r do (fun t => umail None (uprog (k m) t)))
+            end;
+        }.    
 
-  Import CTreeNotations.
-  Local Open Scope ctree_scope.
+    CoFixpoint schedule_one(r: fin' n)(system: sys n T) :=
+      Guard (schedule_one' schedule_one r system).
 
-  CoFixpoint schedule_one(r: fin' n)(system: sys n T) :=
-    Guard (schedule_one' schedule_one r system).
+    (* Nondeterministic pick which process to start first *)
+    Definition schedule(system: sys n T) :=
+      r <- Ctree.branch n ;;
+      schedule_one r system.
 
-  (* Nondeterministic pick which process to start first *)
-  Definition schedule(system: sys n T) :=
-    r <- Ctree.branch n ;;
-    schedule_one r system.
-
-End ScheduleMsg.
+  End ScheduleMsg.
+End MessageOrderScheduler.
