theories/ITree/Events/Net.v
@@ -2,13 +2,11 @@ From CTree Require Import
   ITree.Core.
 
 From CTree Require Export
+  Utils.Utils
   Events.NetE.
 
-Definition send {n T}: uid n -> uid n -> T -> itree (netE n T) unit :=
-  fun i u p => Itree.trigger (Send i u p).
+Definition send {n T}: fin' n -> T -> itree (netE n T) unit :=
+  fun i p => Itree.trigger (Send i p).
 
-Definition recv {n T}: uid n -> itree (netE n T) (option T) :=
-  fun i => Itree.trigger (Recv i).
-
-Notation retry := (Ret (inl tt)).
-Notation exit := (Ret (inr tt)).
+Definition recv {n T}: itree (netE n T) (option T) :=
+  Itree.trigger Recv.
